module Examples.STLC-Rec.SubjectReduction where

open import Relation.Binary.PropositionalEquality using (_â‰¡_; refl; sym; trans; cong; congâ‚‚; subst; module â‰¡-Reasoning)
open â‰¡-Reasoning
open import Data.List using (List; []; _âˆ·_; drop)
open import Data.List.Relation.Unary.Any using (here; there)
open import Data.Unit using (âŠ¤; tt)
open import Function using () renaming (_âˆ‹_ to _by_)

open import Examples.STLC-Rec.Definitions

ope-pres-âŠ¢ : âˆ€ {e : Âµâ‚ âŠ¢ ğ•–} {t : Âµâ‚ âˆ¶âŠ¢ ğ•–} {Ï : Âµâ‚ â†’áµ£ Âµâ‚‚} â†’
  OPE Ï Î“â‚ Î“â‚‚ â†’
  Î“â‚ âŠ¢ e     âˆ¶ t â†’
  Î“â‚‚ âŠ¢ e â‹¯ Ï âˆ¶ t â‹¯ Ï
ope-pres-âŠ¢               {Ï = Ï} ope (Ï„-` refl)            = Ï„-` (ope-pres-telescope _ ope)
ope-pres-âŠ¢ {t = tâ‚ â‡’ tâ‚‚} {Ï = Ï} ope (Ï„-Î» âŠ¢e)              = Ï„-Î» (subst (_ âŠ¢ _ âˆ¶_) (dist-â†‘-ren tâ‚‚ Ï) (ope-pres-âŠ¢ (ope-keep ope) âŠ¢e))
ope-pres-âŠ¢                       ope (Ï„-Â· âŠ¢eâ‚ âŠ¢eâ‚‚)         = Ï„-Â· (ope-pres-âŠ¢ ope âŠ¢eâ‚) (ope-pres-âŠ¢ ope âŠ¢eâ‚‚)
ope-pres-âŠ¢ {t = ÂµÎ± t} {Ï = Ï}    ope (Ï„-fold âŠ¢e)           = Ï„-fold (subst (_ âŠ¢ _ âˆ¶_) (
                                                               t â‹¯ â¦… ÂµÎ± t â¦† â‹¯ Ï                â‰¡âŸ¨ dist-â¦…â¦†â‚›-â‹¯áµ£ t (ÂµÎ± t) Ï âŸ©
                                                               t â‹¯ Ï â†‘ ğ•¥ â‹¯ â¦… ÂµÎ± (t â‹¯ Ï â†‘ ğ•¥) â¦†  âˆ
                                                             ) (ope-pres-âŠ¢ ope âŠ¢e))
ope-pres-âŠ¢ {Ï = Ï}               ope (Ï„-unfold {t = t} âŠ¢e) = subst (_ âŠ¢ _ âˆ¶_) (
                                                               t â‹¯ (Ï â†‘ ğ•¥) â‹¯ â¦… (ÂµÎ± t) â‹¯ Ï â¦† â‰¡âŸ¨ sym (dist-â¦…â¦†â‚›-â‹¯áµ£ t (ÂµÎ± t) Ï) âŸ©
                                                               t â‹¯ â¦… ÂµÎ± t â¦† â‹¯ Ï             âˆ
                                                             ) (Ï„-unfold (ope-pres-âŠ¢ ope âŠ¢e))

wk-pres-âŠ¢ : âˆ€ {e : Âµ âŠ¢ ğ•–} {t : Âµ âˆ¶âŠ¢ ğ•–} (t' : Âµ âˆ¶âŠ¢ ğ•–) â†’
  Î“â‚‚         âŠ¢ e      âˆ¶ t â†’
  (_,,_ {m = ğ•–} Î“â‚‚ t') âŠ¢ wk _ e âˆ¶ wk _ t
wk-pres-âŠ¢ t âŠ¢v =  ope-pres-âŠ¢ (ope-drop ope-id) âŠ¢v

lift-âŠ¢* : âˆ€ {Ïƒ : Âµâ‚ â†’â‚› Âµâ‚‚} (t : Âµâ‚ âˆ¶âŠ¢ ğ•–) â†’
  Î“â‚‚              âŠ¢*  Ïƒ      âˆ¶ Î“â‚ â†’
  (Î“â‚‚ ,, (t â‹¯ Ïƒ)) âŠ¢* (Ïƒ â†‘ ğ•–) âˆ¶ (Î“â‚ ,, t)
lift-âŠ¢* {Ïƒ = Ïƒ} t âŠ¢Ïƒ (here refl) = Ï„-` (sym (dist-â†‘-sub t Ïƒ))
lift-âŠ¢* {Î“â‚‚ = Î“â‚‚} {Î“â‚ = Î“â‚} {Ïƒ = Ïƒ} t âŠ¢Ïƒ (there x) =
  subst ((Î“â‚‚ ,, (t â‹¯ Ïƒ)) âŠ¢ (Ïƒ _ x â‹¯ wk) âˆ¶_)
        (sym (wk-drop-âˆˆ x (Î“â‚ x) â‹¯ wk â‹¯ (Ïƒ â†‘ ğ•–) â‰¡âŸ¨ dist-â†‘-sub (wk-drop-âˆˆ x (Î“â‚ x)) Ïƒ âŸ©
              wk-drop-âˆˆ x (Î“â‚ x) â‹¯ Ïƒ â‹¯ wk       âˆ))
        (wk-pres-âŠ¢ (t â‹¯ Ïƒ) (âŠ¢Ïƒ x))

sub-pres-âŠ¢ : âˆ€ {Î“â‚ : Ctx Âµâ‚} {Î“â‚‚ : Ctx Âµâ‚‚} {e : Âµâ‚ âŠ¢ ğ•–} {t : Âµâ‚ âˆ¶âŠ¢ ğ•–} {Ïƒ : Âµâ‚ â†’â‚› Âµâ‚‚} â†’
  Î“â‚ âŠ¢ e âˆ¶ t â†’
  Î“â‚‚ âŠ¢* Ïƒ âˆ¶ Î“â‚ â†’
  Î“â‚‚ âŠ¢ e â‹¯ Ïƒ âˆ¶ t â‹¯ Ïƒ
sub-pres-âŠ¢                     (Ï„-` {x = x} refl)    âŠ¢Ïƒ = âŠ¢Ïƒ x
sub-pres-âŠ¢ {Ïƒ = Ïƒ}             (Ï„-Î» {tâ‚‚ = tâ‚‚} âŠ¢e)    âŠ¢Ïƒ = Ï„-Î» (subst (_ âŠ¢ _ âˆ¶_) (dist-â†‘-sub tâ‚‚ Ïƒ) (sub-pres-âŠ¢ âŠ¢e (lift-âŠ¢* _ âŠ¢Ïƒ)) )
sub-pres-âŠ¢                     (Ï„-Â· âŠ¢eâ‚ âŠ¢eâ‚‚)         âŠ¢Ïƒ = Ï„-Â· (sub-pres-âŠ¢ âŠ¢eâ‚ âŠ¢Ïƒ) (sub-pres-âŠ¢ âŠ¢eâ‚‚ âŠ¢Ïƒ)
sub-pres-âŠ¢ {t = ÂµÎ± t} {Ïƒ = Ïƒ}  (Ï„-fold âŠ¢e)           âŠ¢Ïƒ = Ï„-fold (subst (_ âŠ¢ _ âˆ¶_) (
                                                            t â‹¯ â¦… ÂµÎ± t â¦† â‹¯ Ïƒ               â‰¡âŸ¨ dist-â¦…â¦†â‚›-â‹¯â‚› t (ÂµÎ± t) Ïƒ âŸ©
                                                            t â‹¯ Ïƒ â†‘ ğ•¥ â‹¯ â¦… ÂµÎ± (t â‹¯ Ïƒ â†‘ ğ•¥) â¦† âˆ
                                                          ) (sub-pres-âŠ¢ âŠ¢e âŠ¢Ïƒ))
sub-pres-âŠ¢ {Ïƒ = Ïƒ}             (Ï„-unfold {t = t} âŠ¢e) âŠ¢Ïƒ = subst (_ âŠ¢ _ âˆ¶_) (
                                                            t â‹¯ Ïƒ â†‘ ğ•¥ â‹¯ â¦… ÂµÎ± (t â‹¯ Ïƒ â†‘ ğ•¥) â¦† â‰¡âŸ¨ sym (dist-â¦…â¦†â‚›-â‹¯â‚› t (ÂµÎ± t) Ïƒ) âŸ©
                                                            t â‹¯ â¦… ÂµÎ± t â¦† â‹¯ Ïƒ              âˆ
                                                          ) (Ï„-unfold (sub-pres-âŠ¢ âŠ¢e âŠ¢Ïƒ))

_,*_ : âˆ€ {Ïƒ : Âµâ‚ â†’â‚› Âµâ‚‚} {t : Âµâ‚ âˆ¶âŠ¢ ğ•–} â†’
  Î“â‚‚ âŠ¢* Ïƒ âˆ¶ Î“â‚ â†’
  Î“â‚‚ âŠ¢  e âˆ¶ t â‹¯ Ïƒ â†’
  Î“â‚‚ âŠ¢* Ïƒ ,â‚› e âˆ¶ Î“â‚ ,, t
_,*_ {Î“â‚‚ = Î“â‚‚} {e = e} {t = t} âŠ¢Ïƒ âŠ¢e (here refl) = subst (Î“â‚‚ âŠ¢ e âˆ¶_) (sym (wk-cancels-,â‚› t _ _)) âŠ¢e
_,*_ {Î“â‚‚ = Î“â‚‚} {Î“â‚ = Î“â‚} {Ïƒ = Ïƒ} âŠ¢Ïƒ âŠ¢v (there x) = subst (Î“â‚‚ âŠ¢ Ïƒ _ x âˆ¶_) (sym (wk-cancels-,â‚› (wk-drop-âˆˆ x (Î“â‚ x)) _ _)) (âŠ¢Ïƒ x)

âŠ¢*-idâ‚› : Î“ âŠ¢* idâ‚› âˆ¶ Î“
âŠ¢*-idâ‚› {Î“ = Î“} x rewrite â‹¯-idâ‚› (wk-telescope Î“ x) = Ï„-` refl

subâ‚-pres-âŠ¢ : âˆ€ {Î“ : Ctx Âµ} {eâ‚ : ğ•– âˆ· Âµ âŠ¢ ğ•–} {eâ‚‚ : Âµ âŠ¢ ğ•–} {tâ‚‚ : Âµ , ğ•– âˆ¶âŠ¢ ğ•–} {tâ‚ : Âµ âˆ¶âŠ¢ ğ•–} â†’
  Î“ ,, tâ‚ âŠ¢ eâ‚ âˆ¶ tâ‚‚ â†’
  Î“ âŠ¢ eâ‚‚ âˆ¶ tâ‚ â†’
  Î“ âŠ¢ eâ‚ â‹¯ â¦… eâ‚‚ â¦† âˆ¶ tâ‚‚ â‹¯ â¦… eâ‚‚ â¦†
subâ‚-pres-âŠ¢ {Î“ = Î“} {eâ‚‚ = eâ‚‚} âŠ¢eâ‚ âŠ¢eâ‚‚ = sub-pres-âŠ¢ âŠ¢eâ‚ (âŠ¢*-idâ‚› ,* subst (Î“ âŠ¢ eâ‚‚ âˆ¶_) (sym (â‹¯-id _)) âŠ¢eâ‚‚)

subject-reduction :
  Î“ âŠ¢ e âˆ¶ t â†’
  e â†ª e' â†’
  Î“ âŠ¢ e' âˆ¶ t
subject-reduction (Ï„-Â· {tâ‚‚ = tâ‚‚} (Ï„-Î» âŠ¢eâ‚) âŠ¢eâ‚‚) (Î²-â‡’ val-eâ‚‚)         = subst (_ âŠ¢ _ âˆ¶_) (wk-cancels-â¦…â¦†â‚› tâ‚‚ _) (subâ‚-pres-âŠ¢ âŠ¢eâ‚ âŠ¢eâ‚‚)
subject-reduction (Ï„-unfold (Ï„-fold âŠ¢e))        (Î²-Âµ val-e)          = âŠ¢e
subject-reduction (Ï„-Â· âŠ¢eâ‚ âŠ¢eâ‚‚)                 (Î¾-Â·â‚ eâ‚â†ªeâ‚')        = Ï„-Â· (subject-reduction âŠ¢eâ‚ eâ‚â†ªeâ‚') âŠ¢eâ‚‚
subject-reduction (Ï„-Â· âŠ¢eâ‚ âŠ¢eâ‚‚)                 (Î¾-Â·â‚‚ val-eâ‚ eâ‚‚â†ªeâ‚‚') = Ï„-Â· âŠ¢eâ‚ (subject-reduction âŠ¢eâ‚‚ eâ‚‚â†ªeâ‚‚')
subject-reduction (Ï„-fold âŠ¢e)                   (Î¾-fold eâ†ªe')        = Ï„-fold (subject-reduction âŠ¢e eâ†ªe')
subject-reduction (Ï„-unfold âŠ¢e)                 (Î¾-unfold eâ†ªe')      = Ï„-unfold (subject-reduction âŠ¢e eâ†ªe')

subject-reduction* :
  Î“ âŠ¢ e âˆ¶ t â†’
  e â†ª* e' â†’
  Î“ âŠ¢ e' âˆ¶ t
subject-reduction* âŠ¢e â†ª*-refl = âŠ¢e
subject-reduction* âŠ¢e (â†ª*-step eâ‚â†ªeâ‚‚ eâ‚‚â†ª*eâ‚ƒ) = subject-reduction* (subject-reduction âŠ¢e eâ‚â†ªeâ‚‚) eâ‚‚â†ª*eâ‚ƒ
